Switch register scheme to codes

src/Prompt_monad.v
@@ -72,70 +72,73 @@ Local Open Scope Z.
 
 Definition address := N.
 
-Inductive monad reg_type a e :=
-  | Done : a -> monad reg_type a e
+Section WithRegisterType.
+Context {register : Type} {reg_to_type : register -> Type}.
+
+Inductive monad a e :=
+  | Done : a -> monad a e
   (* Read a number of bytes from memory, returned in little endian order,
      with or without a tag.  The first nat specifies the address, the second
      the number of bytes. *)
-  | Read_mem : read_kind -> N -> nat -> (list memory_byte -> monad reg_type a e) -> monad reg_type a e
-  | Read_memt : read_kind -> N -> nat -> ((list memory_byte * bitU) -> monad reg_type a e) -> monad reg_type a e
+  | Read_mem : read_kind -> N -> nat -> (list memory_byte -> monad a e) -> monad a e
+  | Read_memt : read_kind -> N -> nat -> ((list memory_byte * bitU) -> monad a e) -> monad a e
   (* Tell the system a write is imminent, at the given address and with the
      given size. *)
-  | Write_ea : write_kind -> N -> nat -> monad reg_type a e -> monad reg_type a e
+  | Write_ea : write_kind -> N -> nat -> monad a e -> monad a e
   (* Request the result : store-exclusive *)
-  | Excl_res : (bool -> monad reg_type a e) -> monad reg_type a e
+  | Excl_res : (bool -> monad a e) -> monad a e
   (* Request to write a memory value of the given size at the given address,
      with or without a tag. *)
-  | Write_mem : write_kind -> N -> nat -> list memory_byte -> (bool -> monad reg_type a e) -> monad reg_type a e
-  | Write_memt : write_kind -> N -> nat -> list memory_byte -> bitU -> (bool -> monad reg_type a e) -> monad reg_type a e
-  | Write_tag : write_kind -> N -> bitU -> (bool -> monad reg_type a e) -> monad reg_type a e
+  | Write_mem : write_kind -> N -> nat -> list memory_byte -> (bool -> monad a e) -> monad a e
+  | Write_memt : write_kind -> N -> nat -> list memory_byte -> bitU -> (bool -> monad a e) -> monad a e
+  | Write_tag : write_kind -> N -> bitU -> (bool -> monad a e) -> monad a e
   (* Tell the system to dynamically recalculate dependency footprint *)
-  | Footprint : monad reg_type a e -> monad reg_type a e
+  | Footprint : monad a e -> monad a e
   (* Request a memory barrier *)
-  | Barrier : barrier_kind -> monad reg_type a e -> monad reg_type a e
+  | Barrier : barrier_kind -> monad a e -> monad a e
   (* Request to read register, will track dependency when mode.track_values *)
-  | Read_reg : forall T, reg_type T -> (T -> monad reg_type a e) -> monad reg_type a e
+  | Read_reg : forall (r : register), (reg_to_type r -> monad a e) -> monad a e
   (* Request to write register *)
-  | Write_reg : forall T, reg_type T -> T -> monad reg_type a e -> monad reg_type a e
+  | Write_reg : forall (r : register), reg_to_type r -> monad a e -> monad a e
   (* Request to choose a Boolean, e.g. to resolve an undefined bit. The string
      argument may be used to provide information to the system about what the
      Boolean is going to be used for. *)
-  | Choose : string -> forall ty, (choose_type ty -> monad reg_type a e) -> monad reg_type a e
+  | Choose : string -> forall ty, (choose_type ty -> monad a e) -> monad a e
   (* Print debugging or tracing information *)
-  | Print : string -> monad reg_type a e -> monad reg_type a e
+  | Print : string -> monad a e -> monad a e
   (*Result of a failed assert with possible error message to report*)
-  | Fail : string -> monad reg_type a e
+  | Fail : string -> monad a e
   (* Exception of type e *)
-  | Exception : e -> monad reg_type a e.
+  | Exception : e -> monad a e.
 
-Arguments Done [_ _ _].
-Arguments Read_mem [_ _ _].
-Arguments Read_memt [_ _ _].
-Arguments Write_ea [_ _ _].
-Arguments Excl_res [_ _ _].
-Arguments Write_mem [_ _ _].
-Arguments Write_memt [_ _ _].
-Arguments Write_tag [_ _ _].
-Arguments Footprint [_ _ _].
-Arguments Barrier [_ _ _].
-Arguments Read_reg [_ _ _ _].
-Arguments Write_reg [_ _ _ _].
-Arguments Choose [_ _ _].
-Arguments Print [_ _ _].
-Arguments Fail [_ _ _].
-Arguments Exception [_ _ _].
+Arguments Done [_ _].
+Arguments Read_mem [_ _].
+Arguments Read_memt [_ _].
+Arguments Write_ea [_ _].
+Arguments Excl_res [_ _].
+Arguments Write_mem [_ _].
+Arguments Write_memt [_ _].
+Arguments Write_tag [_ _].
+Arguments Footprint [_ _].
+Arguments Barrier [_ _].
+Arguments Read_reg [_ _].
+Arguments Write_reg [_ _].
+Arguments Choose [_ _].
+Arguments Print [_ _].
+Arguments Fail [_ _].
+Arguments Exception [_ _].
 
 (* The injectivity tactic can be confused by dependent types when some of the types
    involved don't quite match syntactically.  Sometimes it's easier to apply a lemma
    to a hypothesis instead. *)
-Lemma Choose_injective {rv A E} s ty (x y : choose_type ty -> monad rv A E) :
+Lemma Choose_injective {A E} s ty (x y : choose_type ty -> monad A E) :
   Choose s ty x = Choose s ty y ->
   x = y.
 intros [=].
 assumption.
 Qed.
 
-Inductive event {reg_type} :=
+Inductive event :=
   | E_read_mem : read_kind -> N -> nat -> list memory_byte -> event
   | E_read_memt : read_kind -> N -> nat -> (list memory_byte * bitU) -> event
   | E_write_mem : write_kind -> N -> nat -> list memory_byte -> bool -> event
@@ -145,19 +148,19 @@ Inductive event {reg_type} :=
   | E_excl_res : bool -> event
   | E_barrier : barrier_kind -> event
   | E_footprint : event
-  | E_read_reg : forall {T}, reg_type T -> T -> event
-  | E_write_reg : forall {T}, reg_type T -> T -> event
+  | E_read_reg : forall (r : register), reg_to_type r -> event
+  | E_write_reg : forall (r : register), reg_to_type r -> event
   | E_choose : string -> forall ty, choose_type ty -> event
   | E_print : string -> event.
 Arguments event : clear implicits.
 
-Definition trace regval := list (event regval).
+Definition trace := list event.
 
 (*val return : forall rv a e. a -> monad rv a e*)
-Definition returnm {rv A E} (a : A) : monad rv A E := Done a.
+Definition returnm {A E} (a : A) : monad A E := Done a.
 
 (*val bind : forall rv a b e. monad rv a e -> (a -> monad rv b e) -> monad rv b e*)
-Fixpoint bind {rv A B E} (m : monad rv A E) (f : A -> monad rv B E) := match m with
+Fixpoint bind {A B E} (m : monad A E) (f : A -> monad B E) := match m with
   | Done a => f a
   | Read_mem rk a sz k =>       Read_mem rk a sz       (fun v => bind (k v) f)
   | Read_memt rk a sz k =>      Read_memt rk a sz      (fun v => bind (k v) f)
@@ -176,17 +179,15 @@ Fixpoint bind {rv A B E} (m : monad rv A E) (f : A -> monad rv B E) := match m w
   | Exception e =>              Exception e
 end.
 
-Notation "m >>= f" := (bind m f) (at level 50, left associativity).
 (*val (>>) : forall rv b e. monad rv unit e -> monad rv b e -> monad rv b e*)
-Definition bind0 {rv A E} (m : monad rv unit E) (n : monad rv A E) :=
-  m >>= fun (_ : unit) => n.
-Notation "m >> n" := (bind0 m n) (at level 50, left associativity).
+Definition bind0 {A E} (m : monad unit E) (n : monad A E) :=
+  bind m (fun (_ : unit) => n).
 
 (*val exit : forall rv a e. unit -> monad rv a e*)
-Definition exit {rv A E} (_ : unit) : monad rv A E := Fail "exit".
+Definition exit {A E} (_ : unit) : monad A E := Fail "exit".
 
 (*val maybe_fail : forall 'rv 'a 'e. string -> maybe 'a -> monad 'rv 'a 'e*)
-Definition maybe_fail {rv A E} msg (x : option A) : monad rv A E :=
+Definition maybe_fail {A E} msg (x : option A) : monad A E :=
 match x with
   | Some a => returnm a
   | None => Fail msg
@@ -195,44 +196,43 @@ end.
 (* Helper for value definitions that may contain an assertion or incomplete pattern match.  If the
    computation reduces immediately to a value it will return that, otherwise there will be a
    typechecking failure. *)
-Definition unwrap_value {rv A E} (m : monad rv A E) : match m with Done _ => A | _ => True end :=
+Definition unwrap_value {A E} (m : monad A E) : match m with Done _ => A | _ => True end :=
   match m with
   | Done a => a
   | _ => I
   end.
 
 Section Choose.
-Context {rt : Type -> Type} {E : Type}.
+Context {E : Type}.
 
-Definition choose_bool descr : monad rt bool E := Choose descr ChooseBool returnm.
-Definition choose_bit descr : monad rt bitU E := Choose descr ChooseBit returnm.
-Definition choose_int descr : monad rt Z E := Choose descr ChooseInt returnm.
-Definition choose_nat descr : monad rt Z E := Choose descr ChooseNat returnm.
-Definition choose_real descr : monad rt _ E := Choose descr ChooseReal returnm.
-Definition choose_string descr : monad rt string E := Choose descr ChooseString returnm.
-Definition choose_range descr lo hi : monad rt Z E :=
+Definition choose_bool descr : monad bool E := Choose descr ChooseBool returnm.
+Definition choose_bit descr : monad bitU E := Choose descr ChooseBit returnm.
+Definition choose_int descr : monad Z E := Choose descr ChooseInt returnm.
+Definition choose_nat descr : monad Z E := Choose descr ChooseNat returnm.
+Definition choose_real descr : monad _ E := Choose descr ChooseReal returnm.
+Definition choose_string descr : monad string E := Choose descr ChooseString returnm.
+Definition choose_range descr lo hi : monad Z E :=
   if lo <=? hi
   then Choose descr (ChooseRange lo hi) (fun v => if sumbool_of_bool ((lo <=? v) && (v <=? hi)) then returnm v else Fail "choose_range: Bad value")
   else Fail "choose_range: Bad range".
-Definition choose_bitvector descr n : monad rt (mword n) E := Choose descr (ChooseBitvector n) returnm.
+Definition choose_bitvector descr n : monad (mword n) E := Choose descr (ChooseBitvector n) returnm.
 
 End Choose.
 
 (*val assert_exp : forall rv e. bool -> string -> monad rv unit e*)
-Definition assert_exp {rv E} (exp :bool) msg : monad rv unit E :=
+Definition assert_exp {E} (exp :bool) msg : monad unit E :=
  if exp then Done tt else Fail msg.
 
-Definition assert_exp' {rv E} (exp :bool) msg : monad rv (exp = true) E :=
- if exp return monad rv (exp = true) E then Done eq_refl else Fail msg.
-Definition bindH {rv A P E} (m : monad rv P E) (n : monad rv A E) :=
-  m >>= fun (H : P) => n.
-Notation "m >>> n" := (bindH m n) (at level 50, left associativity).
+Definition assert_exp' {E} (exp :bool) msg : monad (exp = true) E :=
+ if exp return monad (exp = true) E then Done eq_refl else Fail msg.
+Definition bindH {A P E} (m : monad P E) (n : monad A E) :=
+  bind m (fun (H : P) => n).
 
 (*val throw : forall rv a e. e -> monad rv a e*)
-Definition throw {rv A E} e : monad rv A E := Exception e.
+Definition throw {A E} e : monad A E := Exception e.
 
 (*val try_catch : forall rv a e1 e2. monad rv a e1 -> (e1 -> monad rv a e2) -> monad rv a e2*)
-Fixpoint try_catch {rv A E1 E2} (m : monad rv A E1) (h : E1 -> monad rv A E2) := match m with
+Fixpoint try_catch {A E1 E2} (m : monad A E1) (h : E1 -> monad A E2) := match m with
   | Done a =>                   Done a
   | Read_mem rk a sz k =>       Read_mem rk a sz       (fun v => try_catch (k v) h)
   | Read_memt rk a sz k =>      Read_memt rk a sz      (fun v => try_catch (k v) h)
@@ -254,13 +254,13 @@ end.
 (* For early return, we abuse exceptions by throwing and catching
    the return value. The exception type is "either r e", where "inr e"
    represents a proper exception and "inl r" an early return : value "r". *)
-Definition monadR rv a r e := monad rv a (sum r e).
+Definition monadR a r e := monad a (sum r e).
 
 (*val early_return : forall rv a r e. r -> monadR rv a r e*)
-Definition early_return {rv A R E} (r : R) : monadR rv A R E := throw (inl r).
+Definition early_return {A R E} (r : R) : monadR A R E := throw (inl r).
 
 (*val catch_early_return : forall rv a e. monadR rv a a e -> monad rv a e*)
-Definition catch_early_return {rv A E} (m : monadR rv A A E) :=
+Definition catch_early_return {A E} (m : monadR A A E) :=
   try_catch m
     (fun r => match r with
       | inl a => returnm a
@@ -275,16 +275,13 @@ Definition pure_early_return_bind {A B E} (v : E + A) (f : A -> E + B) : E + B :
   | inr a => f a
   end.
 
-Notation "m >>$= f" := (pure_early_return_bind m f) (at level 50, left associativity).
-Notation "m >>$ n" := (m >>$= fun _ => n) (at level 50, left associativity).
-
 Definition pure_early_return {A} (v : A + A) : A :=
   match v with
   | inl v' => v'
   | inr v' => v'
   end.
 
-Definition pure_early_return_embed {rv A R E} (v : R + A) : monadR rv A R E :=
+Definition pure_early_return_embed {A R E} (v : R + A) : monadR A R E :=
   match v with
   | inl v' => early_return v'
   | inr v' => Done v'
@@ -292,12 +289,12 @@ Definition pure_early_return_embed {rv A R E} (v : R + A) : monadR rv A R E :=
 
 (* Lift to monad with early return by wrapping exceptions *)
 (*val liftR : forall rv a r e. monad rv a e -> monadR rv a r e*)
-Definition liftR {rv A R E} (m : monad rv A E) : monadR rv A R E :=
+Definition liftR {A R E} (m : monad A E) : monadR A R E :=
  try_catch m (fun e => throw (inr e)).
 
 (* Catch exceptions in the presence : early returns *)
 (*val try_catchR : forall rv a r e1 e2. monadR rv a r e1 -> (e1 -> monadR rv a r e2) ->  monadR rv a r e2*)
-Definition try_catchR {rv A R E1 E2} (m : monadR rv A R E1) (h : E1 -> monadR rv A R E2) :=
+Definition try_catchR {A R E1 E2} (m : monadR A R E1) (h : E1 -> monadR A R E2) :=
   try_catch m
     (fun r => match r with
       | inl r => throw (inl r)
@@ -305,11 +302,11 @@ Definition try_catchR {rv A R E1 E2} (m : monadR rv A R E1) (h : E1 -> monadR rv
      end).
 
 (*val read_memt_bytes : forall 'rv 'a 'b 'e. Bitvector 'a, Bitvector 'b => read_kind -> 'a -> integer -> monad 'rv (list memory_byte * bitU) 'e*)
-Definition read_memt_bytes {rv A E} rk (addr : mword A) sz : monad rv (list memory_byte * bitU) E :=
+Definition read_memt_bytes {A E} rk (addr : mword A) sz : monad (list memory_byte * bitU) E :=
   Read_memt rk (mword_to_N addr) (Z.to_nat sz) returnm.
 
 (*val read_memt : forall 'rv 'a 'b 'e. Bitvector 'a, Bitvector 'b => read_kind -> 'a -> integer -> monad 'rv ('b * bitU) 'e*)
-Definition read_memt {rv A E} rk (addr : mword A) sz : monad rv (mword (8 * sz) * bitU) E :=
+Definition read_memt {A E} rk (addr : mword A) sz : monad (mword (8 * sz) * bitU) E :=
   bind
     (read_memt_bytes rk addr sz)
     (fun '(bytes, tag) =>
@@ -319,27 +316,27 @@ Definition read_memt {rv A E} rk (addr : mword A) sz : monad rv (mword (8 * sz) 
        end).
 
 (*val read_mem_bytes : forall 'rv 'a 'b 'e. Bitvector 'a, Bitvector 'b => read_kind -> 'a -> integer -> monad 'rv (list memory_byte) 'e*)
-Definition read_mem_bytes {rv A E} rk (addr : mword A) sz : monad rv (list memory_byte) E :=
+Definition read_mem_bytes {A E} rk (addr : mword A) sz : monad (list memory_byte) E :=
   Read_mem rk (mword_to_N addr) (Z.to_nat sz) returnm.
 
 (*val read_mem : forall 'rv 'a 'b 'e. Bitvector 'a, Bitvector 'b => read_kind -> 'a -> integer -> monad 'rv 'b 'e*)
-Definition read_mem {rv A E} rk (addrsz : Z) (addr : mword A) sz : monad rv (mword (8 * sz)) E :=
+Definition read_mem {A E} rk (addrsz : Z) (addr : mword A) sz : monad (mword (8 * sz)) E :=
   bind
     (read_mem_bytes rk addr sz)
     (fun bytes =>
        maybe_fail "bits_of_mem_bytes" (of_bits (bits_of_mem_bytes bytes))).
 
 (*val excl_result : forall rv e. unit -> monad rv bool e*)
-Definition excl_result {rv e} (_:unit) : monad rv bool e :=
+Definition excl_result {e} (_:unit) : monad bool e :=
   let k successful := (returnm successful) in
   Excl_res k.
 
-Definition write_mem_ea {rv a E} wk (addrsz : Z) (addr: mword a) sz : monad rv unit E :=
+Definition write_mem_ea {a E} wk (addrsz : Z) (addr: mword a) sz : monad unit E :=
  Write_ea wk (mword_to_N addr) (Z.to_nat sz) (Done tt).
 
 (*val write_mem : forall 'rv 'a 'b 'e. Bitvector 'a, Bitvector 'b =>
   write_kind -> integer -> 'a -> integer -> 'b -> monad 'rv bool 'e*)
-Definition write_mem {rv a E} wk (addrsz : Z) (addr : mword a) sz (v : mword (8 * sz)) : monad rv bool E :=
+Definition write_mem {a E} wk (addrsz : Z) (addr : mword a) sz (v : mword (8 * sz)) : monad bool E :=
   match (mem_bytes_of_bits v, mword_to_N addr) with
     | (Some v, addr) =>
        Write_mem wk addr (Z.to_nat sz) v returnm
@@ -348,56 +345,55 @@ Definition write_mem {rv a E} wk (addrsz : Z) (addr : mword a) sz (v : mword (8 
 
 (*val write_memt : forall 'rv 'a 'b 'e. Bitvector 'a, Bitvector 'b =>
   write_kind -> 'a -> integer -> 'b -> bitU -> monad 'rv bool 'e*)
-Definition write_memt {rv a E} wk (addr : mword a) sz (v : mword (8 * sz)) tag : monad rv bool E :=
+Definition write_memt {a E} wk (addr : mword a) sz (v : mword (8 * sz)) tag : monad bool E :=
   match (mem_bytes_of_bits v, mword_to_N addr) with
     | (Some v, addr) =>
        Write_memt wk addr (Z.to_nat sz) v tag returnm
     | _ => Fail "write_mem"
   end.
 
-Definition write_tag {rv a E} wk (addr : mword a) tag : monad rv bool E :=
+Definition write_tag {a E} wk (addr : mword a) tag : monad bool E :=
   let addr := mword_to_N addr in
        Write_tag wk addr tag returnm.
 
 (* This alternate version is used in a few places, but should probably disappear *)
-Definition write_tag_bool {rv a E} (addr : mword a) tag : monad rv bool E :=
+Definition write_tag_bool {a E} (addr : mword a) tag : monad bool E :=
   let addr := mword_to_N addr in
        Write_tag Write_plain addr (bitU_of_bool tag) returnm.
 
-Definition read_reg {rt a e} (reg : rt a) : monad rt a e :=
+Definition read_reg {e} (reg : register) : monad (reg_to_type reg) e :=
   let k v := Done v in
   Read_reg reg k.
 
-Definition read_reg_ref {rt a e} (ref : register_ref rt a) : monad rt a e :=
-  let k v := Done v in
+Definition read_reg_ref {a e} (ref : @register_ref register reg_to_type a) : monad a e :=
+  let k v := Done (ref.(to_ty) v) in
   Read_reg ref.(reg) k.
 
-Definition reg_deref {rt a e} := @read_reg_ref rt a e.
+Definition reg_deref {a e} := @read_reg_ref a e.
 
-Definition write_reg {rt a e} (reg : rt a) (v : a) : monad rt unit e :=
+Definition write_reg {e} (reg : register) (v : reg_to_type reg) : monad unit e :=
  Write_reg reg v (Done tt).
 
-Definition write_reg_ref {rt a e} (ref : register_ref rt a) (v : a) : monad rt unit e :=
- Write_reg ref.(reg) v (Done tt).
+Definition write_reg_ref {a e} (ref : @register_ref register reg_to_type a) (v : a) : monad unit e :=
+ Write_reg ref.(reg) (ref.(from_ty) v) (Done tt).
 
 (*val barrier : forall rv e. barrier_kind -> monad rv unit e*)
-Definition barrier {rv e} bk : monad rv unit e := Barrier bk (Done tt).
+Definition barrier {e} bk : monad unit e := Barrier bk (Done tt).
 
 (*val footprint : forall rv e. unit -> monad rv unit e*)
-Definition footprint {rv e} (_ : unit) : monad rv unit e := Footprint (Done tt).
+Definition footprint {e} (_ : unit) : monad unit e := Footprint (Done tt).
 
 (* Event traces *)
 
 Section EventTraces.
 
-Context (register : Type -> Type).
-Context (register_eq_cast : forall {T T'} (P : Type -> Type) (r : register T) (r' : register T'), P T -> option (P T')).
-Context (regval_eqb : forall {T} (r : register T), T -> T -> bool).
+Context (register_eq_cast : forall (P : Type -> Type) (r r' : register), P (reg_to_type r) -> option (P (reg_to_type r'))).
+Context (regval_eqb : forall (r : register), reg_to_type r -> reg_to_type r -> bool).
 
 Local Open Scope bool_scope.
 
 (*val emitEvent : forall 'regval 'a 'e. Eq 'regval => monad 'regval 'a 'e -> event 'regval -> maybe (monad 'regval 'a 'e)*)
-Definition emitEvent {A E}  (m : monad register A E) (e : event register) : option (monad register A E) :=
+Definition emitEvent {A E}  (m : monad A E) (e : event) : option (monad A E) :=
  match (e, m) with
   | (E_read_mem rk a sz v, Read_mem rk' a' sz' k) =>
      if read_kind_beq rk' rk && N.eqb a' a && Nat.eqb sz' sz then Some (k v) else None
@@ -408,13 +404,13 @@ Definition emitEvent {A E}  (m : monad register A E) (e : event register) : opti
   | (E_write_memt wk a sz v tag r, Write_memt wk' a' sz' v' tag' k) =>
      if write_kind_beq wk' wk && N.eqb a' a && Nat.eqb sz' sz && generic_eq v' v && generic_eq tag' tag then Some (k r) else None
   | (E_read_reg r v, Read_reg r' k) =>
-     match register_eq_cast _ _ _ r r' v with
+     match register_eq_cast (fun x => x) r r' v with
      | Some v1 => Some (k v1)
      | None => None
      end
-  | (E_write_reg r v, @Write_reg _ _ _ T r' v' k) =>
-     match register_eq_cast _ _ _ r r' v with
-     | Some v1 => if regval_eqb _ r' v' v1 then Some k else None
+  | (E_write_reg r v, @Write_reg _ _ r' v' k) =>
+     match register_eq_cast (fun x => x) r r' v with
+     | Some v1 => if regval_eqb r' v' v1 then Some k else None
      | None => None
      end
   | (E_write_ea wk a sz, Write_ea wk' a' sz' k) =>
@@ -439,13 +435,13 @@ match a with
 | None => None
 end.
 
-Fixpoint runTrace {A E} (t : trace register) (m : monad register A E) : option (monad register A E) :=
+Fixpoint runTrace {A E} (t : trace) (m : monad A E) : option (monad A E) :=
 match t with
   | [] => Some m
   | e :: t' => option_bind (emitEvent m e) (runTrace t')
 end.
 
-Definition final {A E} (m : monad register A E) : bool :=
+Definition final {A E} (m : monad A E) : bool :=
 match m with
   | Done _ => true
   | Fail _ => true
@@ -453,22 +449,48 @@ match m with
   | _ => false
 end.
 
-Definition hasTrace {A E} (t : trace register) (m : monad register A E) : bool :=
+Definition hasTrace {A E} (t : trace) (m : monad A E) : bool :=
 match runTrace t m with
   | Some m => final m
   | None => false
 end.
 
-Definition hasException {A E} (t : trace register) (m : monad register A E) :=
+Definition hasException {A E} (t : trace) (m : monad A E) :=
 match runTrace t m with
   | Some (Exception _) => true
   | _ => false
 end.
 
-Definition hasFailure {A E} (t : trace register) (m : monad register A E) :=
+Definition hasFailure {A E} (t : trace) (m : monad A E) :=
 match runTrace t m with
   | Some (Fail _) => true
   | _ => false
 end.
 
 End EventTraces.
+
+End WithRegisterType.
+
+Notation "m >>= f" := (bind m f) (at level 50, left associativity).
+Notation "m >> n" := (bind0 m n) (at level 50, left associativity).
+Notation "m >>> n" := (bindH m n) (at level 50, left associativity).
+
+Notation "m >>$= f" := (pure_early_return_bind m f) (at level 50, left associativity).
+Notation "m >>$ n" := (m >>$= fun _ => n) (at level 50, left associativity).
+
+Arguments Done [_ _ _ _].
+Arguments Read_mem [_ _ _ _].
+Arguments Read_memt [_ _ _ _].
+Arguments Write_ea [_ _ _ _].
+Arguments Excl_res [_ _ _ _].
+Arguments Write_mem [_ _ _ _].
+Arguments Write_memt [_ _ _ _].
+Arguments Write_tag [_ _ _ _].
+Arguments Footprint [_ _ _ _].
+Arguments Barrier [_ _ _ _].
+Arguments Read_reg [_ _ _ _].
+Arguments Write_reg [_ _ _ _].
+Arguments Choose [_ _ _ _].
+Arguments Print [_ _ _ _].
+Arguments Fail [_ _ _ _].
+Arguments Exception [_ _ _ _].
