src/Operators_mwords.v
@@ -69,7 +69,7 @@ Require Import TypeCasts Values Instances Prompt_monad Prompt MachineWord.
 From Coq Require Import ZArith Lia Eqdep_dec.
 Local Open Scope Z.
 
-Definition autocast_m {rv e m n} {T : Z -> Type} `{H : Inhabited (T n)} (x : monad rv (T m) e) : monad rv (T n) e :=
+Definition autocast_m {rv rt e m n} {T : Z -> Type} `{H : Inhabited (T n)} (x : @monad rv rt (T m) e) : @monad rv rt (T n) e :=
   x >>= fun x => returnm (autocast x).
 
 (*
